theories/CompileCorrect.v
@@ -801,13 +801,14 @@ Section fix_global.
     | Malfunction.Mconvert (from, to, x) => wellformed Γ x
     | Malfunction.Mblock (tag, xs) => Nat.ltb (int_to_nat tag) 200 && forallb (wellformed Γ) xs
     | Malfunction.Mfield (i, x) => wellformed Γ x
+    (* | Malfunction.Mlazy x => wellformed Γ x *)
+    (* | Malfunction.Mforce x => wellformed Γ x *)
     | _ => false
 (*    | Malfunction.Mvecnew (ty, x1, x2) => wellformed Γ x1 && wellformed Γ x2
     | Malfunction.Mvecget (ty, x1, x2) => wellformed Γ x1 && wellformed Γ x2
     | Malfunction.Mvecset (ty, x1, x2, x3) => wellformed Γ x1 && wellformed Γ x2 && wellformed Γ x3
     | Malfunction.Mveclen (ty, x) => false
-    | Malfunction.Mlazy x => wellformed Γ x
-    | Malfunction.Mforce x => wellformed Γ x *)
+     *)
     end
   with wellformed_binding Γ (b : Malfunction.binding) :=
          match b with
@@ -896,10 +897,39 @@ Proof.
       eapply IHl2. lia.
 Qed.
 
+(* We disable primitive arrays and fix/cofix for correctness. *)
+Definition extraction_env_flags_mlf := 
+  let nolazy_array_term_flags := {|
+    EWellformed.has_tBox := false;
+    EWellformed.has_tRel := true;
+    EWellformed.has_tVar := false;
+    EWellformed.has_tEvar := false;
+    EWellformed.has_tLambda := true;
+    EWellformed.has_tLetIn := true;
+    EWellformed.has_tApp := true;
+    EWellformed.has_tConst := true;
+    EWellformed.has_tConstruct := true;
+    EWellformed.has_tCase := true;
+    EWellformed.has_tProj := false;
+    EWellformed.has_tFix := true;
+    EWellformed.has_tCoFix := false;
+    EWellformed.has_tPrim := 
+      {| EWellformed.has_primint := true;
+         EWellformed.has_primfloat := true;
+         EWellformed.has_primarray := false |};
+    EWellformed.has_tLazy_Force := false
+  |}
+  in
+  {|
+  EWellformed.has_axioms := false;
+  EWellformed.has_cstr_params := false;
+  EWellformed.term_switches := nolazy_array_term_flags;
+  EWellformed.cstr_as_blocks := true |}.
+
 Lemma compile_wellformed Γ n s t (Σ : EAst.global_declarations) :
     (forall i args, lookup_constructor_args Σ i = Some args ->
             blocks_until (List.length args) args < 200) ->
-  EWellformed.wellformed (efl := extraction_env_flags) Σ n t ->
+  EWellformed.wellformed (efl := extraction_env_flags_mlf) Σ n t ->
   represents Γ [] s t ->
   wellformed (map fst (compile_env Σ)) Γ (compile Σ s).
 Proof.
@@ -1038,13 +1068,11 @@ Proof.
       cbn. eapply nth_error_In in Eq.
       eapply in_map_iff; eexists; split; eauto.
   - depelim X; eauto. subst a0.
-    simp compile; cbn.
-    unfold EPrimitive.prim_array. simp compile.
-    cbn. todo "arrays".
+    now simp compile; cbn in Hwf |- *.
 Qed.
 
 Lemma compile_extends Γ n s t (Σ Σ' : EAst.global_declarations) :
-  EWellformed.wellformed (efl := extraction_env_flags) Σ n t ->
+  EWellformed.wellformed (efl := extraction_env_flags_mlf) Σ n t ->
   represents Γ [] s t ->
   EGlobalEnv.extends Σ Σ' ->
   compile Σ s = compile Σ' s.
@@ -1102,10 +1130,12 @@ Proof.
       f_equal; eauto. f_equal; eauto. unshelve eapply (IHa0 _ _ (S n)); eauto.
       replace (#|l'| + S n) with (S (#|l'| + n)) by lia. eauto.
   - destruct p as [? []]; simp compile; eauto.
-    depelim X. specialize (e eq_refl). cbn in Hwf.
-    f_equal. f_equal. rewrite !map_InP_spec; cbn.
+    depelim X. specialize (e eq_refl). now cbn in Hwf.
+    (*f_equal. f_equal. rewrite !map_InP_spec; cbn.
     subst a' a1; cbn in *. apply andb_and in Hwf as []. cbn in *. f_equal; eauto.
-    todo "arrays". f_equal. eapply e; tea.
+    f_equal. eapply e; tea.*)
+  - f_equal; rtoProp; intuition eauto.
+  - f_equal; rtoProp; intuition eauto.
 Qed.  
 
 Lemma Mapply_eval_fail `{Heap} globals locals 
