theories/Pipeline.v
@@ -397,9 +397,10 @@ Program Definition compile_to_malfunction (efl := named_extraction_env_flags) `{
       obseq p _ p' v v' := forall (hh:heap), v' = CompileCorrect.compile_value p.1 v
   |}.
 Next Obligation. sq.
-  erewrite map_ext.
-  eapply compile_wellformed.
-  eapply H3. eapply H4. eapply H5.
+  erewrite (map_ext _ fst).
+  eapply (compile_wellformed _ 0 _ H2).
+  eapply H3.
+  apply ECoInductiveToInductive.trust_cofix. (* eapply H4. *) eapply H5.
   intros. now destruct x.
 Qed.
 Next Obligation.
@@ -972,9 +973,10 @@ Section malfunction_pipeline_wellformed.
     revert Happ. set (transform _ _ _). intro. 
     rewrite Happ.  
     destruct H2 as [? [[? [? ?]] ?]]. sq.   
-    eapply compile_extends in H. 2-3: eauto. 
+    eapply (compile_extends _ 0) in H. 2-3: eauto. 
     destruct H3 as [? [[? [? ?]] ?]]. sq.
-    eapply compile_extends in H0. 2-3: eauto.
+    eapply (compile_extends _ 0) in H0. 3: eauto. 
+    2-3:eapply ECoInductiveToInductive.trust_cofix.
     revert H H0. clear. unfold p. clear p.
     repeat set (transform _ _ _). clearbody p p0 p1.
     rewrite compile_equation_7; intros; f_equal; eauto. 
@@ -994,8 +996,9 @@ Section malfunction_pipeline_wellformed.
     destruct_compose; intro; cbn.
     unfold compile_to_malfunction, transform at 1. cbn.  
     epose proof (correctness verified_named_erasure_pipeline) as [? [? [? ?]]]. destruct H2. 
-    eapply compile_wellformed; eauto. 
+    eapply (compile_wellformed _ 0); eauto. 
     eapply few_enough_blocks; eauto.
+    eapply ECoInductiveToInductive.trust_cofix.
   Qed. 
 
   Lemma verified_named_erasure_pipeline_inductive_irrel t' expt'
